sementics.v
@@ -43,26 +43,43 @@ Definition empty_block := {|
 
 (* Get the head element of the BB_block *)
 Definition BB_head (cmds: list cmd) : list cmd :=
-  match basic_block_gen cmds empty_block with
+  match (list_cmd_BB_gen cmd_BB_gen cmds empty_block).(BasicBlocks) with
   | [] => []
   | h :: _ => h.(cmd)
   end.
 
+Definition is_CAsgn (cmd: cmd) : bool :=
+  match cmd with
+  | CAsgn _ _ => true
+  | _ => false
+  end.
 
 
 (* Prove that the adding an CAsgn cmd will have the exact same length, probably useful *)
 Lemma seq_cmd_retains_BB:
     forall (asgn: cmd) (cmds: list cmd) (BB_now: BasicBlock),
-        is_seq_cmds (BB_head cmds) = true ->
-        is_seq_cmds [asgn] = true ->
-        cmd_list_len cmd_len (BB_head cmds) > 1 -> 
-        length (basic_block_gen (asgn :: cmds) BB_now) = length (basic_block_gen cmds BB_now).
+        is_CAsgn asgn = true ->
+        ((list_cmd_BB_gen cmd_BB_gen ([asgn] ++ cmds) BB_now).(current_block_num)) = ((list_cmd_BB_gen cmd_BB_gen cmds BB_now).(current_block_num)).
 Proof.
   intros.
   induction cmds.
-  - simpl. 
-    unfold basic_block_gen. 
-    unfold is_seq_cmds in H0.
+  * induction asgn; unfold is_CAsgn in H.
+    - unfold list_cmd_BB_gen.
+      simpl; reflexivity.
+    - discriminate.
+    - discriminate.
+  * induction asgn; unfold is_CAsgn in H.
+    - unfold list_cmd_BB_gen at 1.
+      simpl.
+      unfold list_cmd_BB_gen at 1 in IHcmds.
+      induction cmds in IHcmds.
+      +  
+
+    - discriminate.
+    - discriminate.
+Qed.
+  
+
   Admitted.
     
 
@@ -84,10 +101,10 @@ Theorem seq_cmds_single_BB:
     forall (cmds : list cmd),        
         is_seq_cmds cmds = true ->
         cmd_list_len cmd_len cmds > 0 -> 
-        length (basic_block_gen cmds empty_block) = 1.
+        length (list_cmd_BB_gen cmds empty_block) = 1.
 Proof.
   intros.
-  unfold basic_block_gen.
+  unfold list_cmd_BB_gen.
   induction cmds.
   - simpl. reflexivity.
   - intros. simpl.
@@ -109,7 +126,7 @@ Theorem seq_cmds_sound:
 Proof. 
   intros.
   unfold BB_head.
-  unfold basic_block_gen.
+  unfold list_cmd_BB_gen.
   induction cmds.
   - simpl. reflexivity.
   - simpl.
