temp.v
@@ -1,0 +1,25 @@
+Require Import Coq.Strings.String.
+Require Import Coq.Lists.List.
+Import ListNotations.
+Require Import Main.grammer.
+Require Import Coq.Program.Wf.
+Require Export String.
+Require Export ZArith.
+Require Export Znumtheory.
+Require Export List.
+Require Export Bool.
+Require Export Lia.
+Open Scope nat.
+
+
+Program Fixpoint bla (n:nat) {measure n} :=
+match n with
+| 0 => 0
+| S n' => S (bla n')
+end.
+
+Lemma obvious: forall n, bla n = n. 
+induction n. reflexivity.
+(* I'm stuck here. For a normal fixpoint, I could for instance use 
+simpl. rewrite IHn. reflexivity. But here, I couldn't find a tactic 
+transforming bla (S n) to S (bla n).*)
